\documentclass[12pt]{article}
\usepackage{zpj}
\newcommand{\poi}[1]{\pp p_{#1}}
\begin{document}
\title{Jacobi Identity for Classical Possion Bracket}
\author{Peijun Zhu}
\maketitle

Definition of Classical Possion Bracket:
\[ [f, g]=\sum_{i=1, 2,\ldots, n}\frac{\pp(f, g)}{\pp(p_i, q_i)}=\sum_{i=1, 2,\ldots, n}\left(\frac{\pp f}{\pp p_i}\frac{\pp g}{\pp q_i}-\frac{\pp f}{\pp q_i}\frac{\pp g}{\pp p_i}\right)\]

If we define $p_{-i}\mdef q_{i}$, and $I=\{\pm 1, \pm, 2,\ldots, \pm n\}$, we can rewrite it:
\[ [f, g]=\sum_{i\in I} \sgn(i) \frac{\pp f}{\pp p_i}\frac{\pp g}{\pp p_{-i}}\]

Jacobi Identity is $[f,[g,h]]+[g,[h,f]]+[h,[f,g]]=0$. With the new notation, we can rewrite it as
\begin{align}
\sum_{\overrightarrow{fgh}}[f,[g,h]]
  &=\sum_{\overrightarrow{fgh}}\sum_{i\in I}\sgn(i)\frac{\pp f}{\pp p_i}\frac{\pp}{\pp p_{-i}}\left(\sum_{j\in I}\sgn(j)\frac{\pp g}{\pp p_j}\frac{\pp h}{\pp p_{-j}}\right)\\
 &=\sum_{\overrightarrow{fgh}}\sum_{i, j\in I}\sgn(ij)\left(\frac{\pp f}{\poi{i}}\frac{\pp h}{\poi{-j}}\frac{\pp^2g}{\poi{-i}\poi{j}}
 +\frac{\pp f}{\poi{i}}\frac{\pp g}{\poi{j}}\frac{\pp^2h}{\poi{-i}\poi{-j}}\right)\\
 &=\sum_{\overrightarrow{fgh}}\sum_{i, j\in I}\sgn(ij)\left(\frac{\pp f}{\poi{i}}\frac{\pp h}{\poi{-j}}\frac{\pp^2g}{\poi{-i}\poi{j}}
 +\frac{\pp h}{\poi{i}}\frac{\pp f}{\poi{j}}\frac{\pp^2g}{\poi{-i}\poi{-j}}\right)\\
 &=\sum_{\overrightarrow{fgh}}\sum_{i, j\in I}\sgn(ij)\left(\frac{\pp f}{\poi{i}}\frac{\pp h}{\poi{-j}}\frac{\pp^2g}{\poi{-i}\poi{j}}
 +\frac{\pp f}{\poi{i}}\frac{\pp h}{\poi{j}}\frac{\pp^2g}{\poi{-i}\poi{-j}}\right)\\
 &=\sum_{\overrightarrow{fgh}}\sum_{i, j\in I}\sgn(ij)\left(\frac{\pp f}{\poi{i}}\frac{\pp h}{\poi{-j}}\frac{\pp^2g}{\poi{-i}\poi{j}}
 -\frac{\pp f}{\poi{i}}\frac{\pp h}{\poi{-j}}\frac{\pp^2g}{\poi{-i}\poi{j}}\right)\\
 &=0
\end{align}

\end{document}
