\documentclass[12pt]{article}
\usepackage{zpj}
\title{Geometrical Optics in Continuum}
\author{\zpj}
\begin{document}
\maketitle
\section{Fermat's Principle}
Fermat's Principle is
\begin{equation}
\delta s=\delta\int n\dd \ell=0
\end{equation}
If we choose the path connecting two points to be
\begin{equation}\bm r=\bm r(t),\quad t_0\leq t\leq t_1\end{equation}
We can write
\begin{equation}
s=\int n\frac{\dd \ell}{\dd t}\dd t, \quad \frac{\dd \ell}{\dd t}=|\dot{\bm r}|
\end{equation}
The Lagrangian about parameter $t$ is
\begin{equation}
L=n\frac{\dd \ell}{\dd t}=n(\bm r)|\bm{\dot r}|
\end{equation}
then the Euler-Lagrange Equation is
\begin{align}
&\left(\frac{\dd}{\dd t}\frac{\pp}{\pp\bm{\dot r}}-\frac{\pp}{\pp\bm{r}}\right)L=0\\
\bm p&=\frac{\pp L}{\pp \bm{\dot r}}=n \hat\tau,\quad\hat{\tau}=\frac{\pp |\dot{\bm r}|}{\pp \bm{\dot r}}=\bm{\dot r}/|\bm{\dot r}|=\frac{\dd\bm r}{\dd\ell}\\
\frac{\dd \bm p}{\dd t}&=\frac{\pp L}{\pp \bm{r}}=\frac{\dd\ell}{\dd t}\nabla n\\
\frac{\dd \bm p}{\dd \ell}&=\nabla n=\bm F
\end{align}
Generalized Momentum $\bm p$ is independent of the choice of $t$, and 
%i.e. \begin{equation}
%n\frac{\dd \hat\tau}{\dd \ell}=\nabla n-\hat{\tau}\frac{\dd n}{\dd \ell}=\left(1-\hat{\tau}\hat{\tau}^T\right)\nabla n=\nabla_\perp n\label{tt}
%\end{equation}
%also
%\begin{equation}
%\frac{\dd \hat\tau}{\dd \ell}=\nabla_\perp n/n=\nabla_\perp \ln n
%\end{equation}
\section{Examples}
\subsection{Rectangular Coordinates}
\begin{equation}
	n(x,y,z)=f(x,y),\quad\bm F=\frac{\pp f}{\pp x}\hat x+\frac{\pp f}{\pp y}\hat y
\end{equation}
It is obvious that $p_z$ are conserved.
\subsection{Central Gradient}
Define $\bm L=\bm r\times \bm p$,
\begin{align}
	\frac{\dd \bm L}{\dd \ell}&=\frac{\dd\bm r}{\dd \ell}\times\bm p+\bm r\times\frac{\dd\bm p}{\dd \ell}
	\\&=\hat{\tau}\times \bm p+\bm r\times\bm F
	\\&=\bm r\times\bm F
\end{align}
$\bm L$ is conserved for a spherical symmetric distribution
\begin{equation}
n(\bm r)=f(r),\quad \bm r\times\bm F=\bm 0
\end{equation}
$L_z$ is conserved for 
\begin{equation}
n(\bm r)=f(r,\theta),\quad (\bm r\times\bm F)_z=0
\end{equation}

\end{document}